Neighborhood/Semantics/Example/Frame4_11259170869739560.lean
@@ -32,6 +32,21 @@ lemma frame_4_11259170869739560.not_valid_axiomM [DecidableEq α] (hab : a ≠ b
       simp [Frame.box, frame_4_11259170869739560, Set.ext_iff, Ne.symm hab]
       decide⟩
 
+instance : frame_4_11259170869739560.NotContainsEmpty := ⟨fun x => by
+  simp only [Set.mem_insert_iff, Set.mem_singleton_iff, not_or]
+  refine ⟨fun h => ?_, fun h => ?_⟩ <;> · have := Set.ext_iff.mp h 0; simp at this⟩
+
+instance : frame_4_11259170869739560.IsSerial where
+  serial X w hw := by
+    simp only [Frame.box, frame_4_11259170869739560, Set.mem_setOf_eq, Set.mem_insert_iff,
+      Set.mem_singleton_iff] at hw
+    simp only [Frame.dia, Frame.box, frame_4_11259170869739560, Set.mem_compl_iff,
+      Set.mem_setOf_eq, Set.mem_insert_iff, Set.mem_singleton_iff]
+    rcases hw with rfl | rfl <;>
+      · rintro (h | h) <;>
+        · have h3 := Set.ext_iff.mp h 3
+          simp at h3
+
 instance : frame_4_11259170869739560.HasPropertyK where
   K X Y := by
     rintro w ⟨hw₁, hw₂⟩
